scan_lib.v
@@ -1,6 +1,6 @@
 Require Import GPUCSL.
 Set Implicit Arguments.
-
+Require Import Bdiv.
 Fixpoint sum_of (s len : nat) (f : nat -> Z) :=
   match len with
     | O => 0
@@ -643,3 +643,140 @@ Proof.
   sep_rewrite_in IHn H. sep_rewrite_in emp_unit_l H; auto.
   sep_rewrite IHn; sep_rewrite emp_unit_l; auto.
 Qed.
+
+
+Lemma low_assn_emp G : low_assn G emp.
+Proof.
+  intros s1 s2 h Hl; split; intros H; exact H.
+Qed.
+
+Lemma low_assn_mp G E1 E2 q :
+  typing_lexp G E1 Lo ->
+  typing_exp G E2 Lo ->
+  low_assn G (E1 -->p (q, E2)).
+Proof.
+  intros H1 H2 s1 s2 h Hl.
+  simpl; unfold_conn; split; simpl; intros H.
+  erewrite (@low_eq_eq_lexp G E1), (@low_eq_eq_exp G E2); eauto.
+  apply low_eq_sym; auto.
+  apply low_eq_sym; auto.
+  erewrite (@low_eq_eq_lexp G E1), (@low_eq_eq_exp G E2); eauto.
+Qed.
+
+Lemma low_assn_star G P Q : 
+  low_assn G P -> low_assn G Q ->
+  low_assn G (P ** Q).
+Proof.
+  intros HP HQ; unfold "**"; intros s1 s2 h Hl; simpl.
+  specialize (HP s1 s2); specialize (HQ s1 s2); simpl in *.
+  split; intros (ph1 & ph2 & H); exists ph1 ph2.
+  rewrite HP, HQ in H; [exact H|auto..].
+  rewrite HP, HQ; [exact H|auto..].
+Qed.
+
+Lemma low_assn_is_array G E n f : forall s,
+  typing_lexp G E Lo ->
+  CSL.low_assn G (is_array E n f s).
+Proof.
+  induction n; simpl in *; intros s He.
+  - apply low_assn_emp.
+  - apply low_assn_star.
+    apply low_assn_mp.
+    cutrewrite (Lo = join Lo Lo); [|eauto].
+    induction E;
+      [constructor; repeat constructor; inversion He; subst; eauto..].
+    constructor; eauto.
+    constructor.
+    apply IHn; auto.
+Qed.
+
+Lemma low_assn_ex {T : Type} G (P : T -> assn) :
+  (forall x, low_assn G (P x)) ->
+  low_assn G (Ex x, P x).
+Proof.
+  unfold low_assn, indeP.
+  intros Hl s1 s2 h Hlow; simpl.
+  split; intros [x H]; exists x; simpl in *.
+  rewrite Hl.
+  exact H.
+  apply low_eq_sym; eauto.
+  rewrite Hl.
+  exact H.
+  eauto.
+Qed.
+
+Lemma low_assn_pure G P :
+  low_assn G (pure P).
+Proof.
+  intros s1 s2 h Hlow; simpl. unfold Apure; split; auto.
+Qed.
+
+Lemma low_assn_ban G P :
+  low_assn G P ->
+  low_assn G !(P).
+Proof.
+  intros Hl s1 s2 h Hlow; simpl.
+  unfold ban, "//\\"; intros.
+  unfold low_assn, indeP in Hl; simpl in Hl.
+  rewrite Hl; eauto.
+  split; intros H; exact H.
+Qed.
+
+Lemma low_assn_eeq E1 E2 G:
+  typing_exp G E1 Lo ->
+  typing_exp G E2 Lo ->
+  low_assn G (E1 === E2).
+Proof.
+  intros H1 H2; unfold_conn; intros s1 s2 h Hlow; simpl.
+  erewrite (@low_eq_eq_exp G E1); eauto.
+  erewrite (@low_eq_eq_exp G E2); eauto.
+  split; auto.
+Qed.
+
+Definition val := Z.
+
+Definition skip_arr (e : loc_exp) st len skip f_ini i :=
+  nth i (distribute skip e len f_ini (nt_step skip) st) emp. 
+
+Lemma low_assn_skip_arr G E n skip f_ini i : forall st,
+  typing_lexp G E Lo ->
+  low_assn G (skip_arr E st n skip f_ini i).
+Proof.
+  assert (skip = 0 \/ skip <> 0) as [|] by omega.
+  - subst; unfold skip_arr; induction n; simpl in *; intros s He.
+    destruct i; apply low_assn_emp.
+    unfold nt_step; simpl.
+    rewrite nth_overflow; [apply low_assn_emp|].
+    assert (length (distribute 0 E n f_ini (fun _ : nat => 0) (S s)) = 0).
+    { rewrite distribute_length; eauto. }
+    lazymatch goal with [|- context [match ?X with _ => _ end]] => destruct X end;
+      simpl in *; try omega.
+  - unfold skip_arr; induction n; simpl in *; intros s He.
+    + rewrite nth_nseq; destruct leb; apply low_assn_emp.
+    + assert (i < skip \/ skip <= i) as [|] by omega.
+      rewrite nth_add_nth; [|try rewrite distribute_length; unfold nt_step; eauto..].
+      destruct beq_nat.
+      apply low_assn_star; eauto.
+      apply low_assn_mp.
+      cutrewrite (Lo = join Lo Lo); [|eauto].
+      repeat constructor; eauto.
+      constructor.
+      eauto.
+      rewrite nth_overflow; eauto.
+      apply low_assn_emp.
+      rewrite add_nth_length, distribute_length; eauto.
+Qed.
+
+Ltac prove_low_assn :=
+  match goal with
+    | [|- low_assn _ (Ex _, _) ] => apply low_assn_ex; intros
+    | [|- low_assn _ (_ ** _) ] => apply low_assn_star
+    | [|- low_assn _ ( !(_) ) ] => apply low_assn_ban
+    | [|- low_assn _ ( _ === _) ] => apply low_assn_eeq
+    | [|- low_assn _ (pure _) ] => apply low_assn_pure
+    | [|- low_assn _ (if ?X then _ else _) ] => destruct X
+    | [|- low_assn _ (is_array _ _ _ _) ] => apply low_assn_is_array
+    | [|- low_assn _ emp ] => apply low_assn_emp
+    | [|- low_assn _ (is_array _ _ _ _ _ _) ] => apply low_assn_is_array
+    | _ => now (unfold low_assn, indeP; intros; tauto)
+  end.
